\documentclass[a4paper]{scrartcl}
\usepackage{amsmath} 

\title{Important ML formulas}
\date{}

\begin{document}
\maketitle

\section{Gaussians}

Definition:

\begin{align}
    \mathcal{N}(x|\mu, C) &= \frac{1}{|C| (2 \pi)^{d/2}} \exp\left[ -\frac{1}{2} (x - \mu)^T C^{-1} (c - \mu) \right]
\end{align}

Marginals and conditionals (see Bishop, (2.113) - (2.117)):
    
\begin{align}
    p(x) &= \mathcal{N}(x|\mu, \Lambda^{-1}) \\
    p(y|x) &= \mathcal{N}(y|A x + b, L^{-1}) \\
    p(y) &= \int \mathrm{d}x\; p(y|x)p(x) 
        = \mathcal{N}(y|A\mu + b, L^{-1} + A \Lambda^{-1} A^T) \\
    p(x|y) &= \frac{p(y|x)p(x)}{p(y)} 
        = \mathcal{N}(y|\Sigma \left\{ A^T L (y - b) + \Lambda \mu \right\}, \Sigma) \\
    \Sigma &= \left( \Lambda  + A^T L A \right)^{-1}
\end{align}

Conditioning on blocks

\begin{align}
    p(x) &= \mathcal{N}(x|\mu, C) \\
    C &= \begin{pmatrix}
        C_N & k \\
        k^T & c
    \end{pmatrix} \\
    x &= (x_N, x_{N+1})^T \\
    \mu &= (\mu_N, \mu_{N+1})^T
\end{align}

Then:

\begin{align}
    p(x_{N+1}|x_{N}) &= 
        \mathcal{N}\left( x_{N+1} | \tilde{\mu}_{N+1}, \tilde{C}_{N+1} \right) \\
    \tilde{\mu}_{N+1} &= \mu_{N+1} + k^T C_N^{-1} (x_N - \mu_N) \\
    \tilde{C}_{N+1} &= c - k^T C_N^{-1} k
\end{align}

\section{Laplace approximation}
\begin{align}
    \log p(x) 
        &\approx \log p(x^\star) + \frac{1}{2} \left(x - x^\star \right)^T H \left(x - x^\star\right) \\
        &= \mathcal{N}(x|x^\star, H^{-1}) \\
    &\left. \frac{\partial}{\partial x} \log p(x) \right|_{x^\star} = 0 \\
    &H_{ij} = \frac{\partial^2}{\partial x_i \partial x_j} \log p(x) 
\end{align}

\section{Sigmoids}
\begin{align}
    \sigma(x) &= \frac{1}{1 - \exp(-x)} \\
    \sigma(-x) &= 1 - \sigma(x)  \\
    \log \frac{\sigma(x)}{1 - \sigma(x)} &= x \\
    \frac{\partial}{\partial x}\sigma(x) &= \sigma(x) (1 - \sigma(x))
\end{align}

\section{Block Matrix Inverse}
\begin{align}
    \begin{bmatrix} 
            A_{00} & A_{01} \\ 
            A_{10} & A_{11} 
    \end{bmatrix}^{-1} 
    &= \begin{bmatrix} 
        A_{00}^{-1} + F E^{-1} G & -F E^{-1} \\ 
        -E^{-1} G & E^{-1} 
    \end{bmatrix} \\
    E &= A_{11} - A_{10} A_{00}^{-1} A_{01} \\
    F &= A_{00}^{-1}A_{01} \\
    G &= A_{10} A_{00}^{-1}
\end{align}

\end{document}